Fix handling of rule constants in MFA framework

ExistentialRules/Terms/ListsOfTerms.lean
@@ -1,40 +1,40 @@
 import ExistentialRules.Terms.Basic
 
-variable {sig : Signature} [DecidableEq sig.C] [DecidableEq sig.V]
-
-def all_term_lists_of_length (candidate_terms : List (GroundTerm sig)) : Nat -> List (List (GroundTerm sig))
+-- TODO: maybe extract this to basic data structures as this is generic for lists
+def all_lists_of_length (candidates : List α) : Nat -> List (List α)
 | .zero => [[]]
 | .succ n =>
-  let prev_terms := all_term_lists_of_length candidate_terms n
-  candidate_terms.flatMap (fun t =>
+  let prev_terms := all_lists_of_length candidates n
+  candidates.flatMap (fun t =>
     prev_terms.map (fun ts =>
       t :: ts
     )
   )
 
-theorem mem_all_term_lists_of_length (candidate_terms : List (GroundTerm sig)) (length : Nat) : ∀ ts, ts ∈ (all_term_lists_of_length candidate_terms length) ↔ (ts.length = length ∧ (∀ t, t ∈ ts -> t ∈ candidate_terms)) := by
+-- TODO: same as above
+theorem mem_all_lists_of_length (candidates : List α) (length : Nat) : ∀ as, as ∈ (all_lists_of_length candidates length) ↔ (as.length = length ∧ (∀ a, a ∈ as -> a ∈ candidates)) := by
   induction length with
-  | zero => intro ts; unfold all_term_lists_of_length; simp; intro eq t _ mem; rw [eq] at mem; simp at mem
+  | zero => intro as; unfold all_lists_of_length; simp; intro eq a mem; rw [eq] at mem; simp at mem
   | succ length ih =>
-    intro ts
-    unfold all_term_lists_of_length
+    intro as
+    unfold all_lists_of_length
     simp only [List.mem_flatMap, List.mem_map]
 
     constructor
     . intro h
-      rcases h with ⟨t, t_mem, prev, prev_mem, ts_eq⟩
-      rw [← ts_eq]
+      rcases h with ⟨a, a_mem, prev, prev_mem, as_eq⟩
+      rw [← as_eq]
       specialize ih prev
       have ih := ih.mp prev_mem
       constructor
       . rw [List.length_cons, ih.left]
-      . intro t' t'_mem
-        rw [List.mem_cons] at t'_mem
-        cases t'_mem with
-        | inl t'_mem => rw [t'_mem]; apply t_mem
-        | inr t'_mem => apply ih.right; exact t'_mem
+      . intro a' a'_mem
+        rw [List.mem_cons] at a'_mem
+        cases a'_mem with
+        | inl a'_mem => rw [a'_mem]; apply a_mem
+        | inr a'_mem => apply ih.right; exact a'_mem
     . intro h
-      cases ts with
+      cases as with
       | nil => simp at h
       | cons hd tl =>
         exists hd
@@ -48,10 +48,12 @@ theorem mem_all_term_lists_of_length (candidate_terms : List (GroundTerm sig)) (
             . have l := h.left
               rw [List.length_cons, Nat.add_right_cancel_iff] at l
               exact l
-            . intro t t_mem
+            . intro a a_mem
               apply h.right
-              simp [t_mem]
+              simp [a_mem]
           . rfl
+
+variable {sig : Signature} [DecidableEq sig.C] [DecidableEq sig.V]
 
 def all_terms_limited_by_depth (constants : List sig.C) (funcs : List (SkolemFS sig)) : Nat -> List (GroundTerm sig)
 | 0 => []
@@ -59,9 +61,9 @@ def all_terms_limited_by_depth (constants : List sig.C) (funcs : List (SkolemFS 
 | .succ (.succ depth) =>
   let prev := all_terms_limited_by_depth constants funcs (.succ depth)
   funcs.flatMap (fun func =>
-    (all_term_lists_of_length prev func.arity).attach.map (fun ⟨ts, mem⟩ =>
+    (all_lists_of_length prev func.arity).attach.map (fun ⟨ts, mem⟩ =>
       GroundTerm.func func ts (by
-        rw [mem_all_term_lists_of_length] at mem
+        rw [mem_all_lists_of_length] at mem
         exact mem.left
       )
     )
@@ -198,7 +200,7 @@ theorem mem_all_terms_limited_by_depth (constants : List sig.C) (funcs : List (S
           unfold List.attachWith at ts_mem
           rw [List.mem_pmap] at ts_mem
           rcases ts_mem with ⟨ts_val, ts_mem, ts_eq⟩
-          rw [mem_all_term_lists_of_length] at ts_mem
+          rw [mem_all_lists_of_length] at ts_mem
 
           rw [GroundTerm.depth_func]
           rw [GroundTerm.constants_func]
@@ -292,8 +294,8 @@ theorem mem_all_terms_limited_by_depth (constants : List sig.C) (funcs : List (S
             . apply funcs_mem
               simp
 
-            have ts_mem : ts ∈ all_term_lists_of_length (all_terms_limited_by_depth constants funcs depth.succ) t_func.arity := by
-              rw [mem_all_term_lists_of_length]
+            have ts_mem : ts ∈ all_lists_of_length (all_terms_limited_by_depth constants funcs depth.succ) t_func.arity := by
+              rw [mem_all_lists_of_length]
               constructor
               . have prop := t.property
                 unfold PreGroundTerm.arity_ok at prop
